F

Clap/Lang/F/F.lean
@@ -16,16 +16,97 @@ def isValid (x : F p) (varStore : VarStore p) : Prop :=
 
 instance : IsValid p (F p) := ⟨fun Γ x ↦ F.isValid x Γ⟩
 
+lemma isValid_iff {varStore : VarStore p} {x : F p} :
+  IsValid.isValid (α := F p) varStore x ↔ (x.eval varStore).isSome
+:= by rfl
+
+lemma isValid_iff_mem {varStore : VarStore p} {x : F p} :
+  IsValid.isValid (α := F p) varStore x ↔ x ∈ varStore
+:= isValid_iff.trans CircuitStateM.mem_iff_isSome.symm
+
+def isAlwaysValid (x : F p) : Prop := ∀ varStore, x.isValid varStore
+
 instance : VarStoreSize p (F p) where
   size := 1
   toLinear Γ x := #v[x.eval Γ |>.getD 42]
 
+def toZMod (x : F p) (varStore : VarStore p) : Option (ZMod p) := x.eval varStore
+def ofZMod (p : ℕ) (v : ZMod p) : F p := .c v
+
+@[simp, grind =]
+lemma toZMod_def {varStore : VarStore p} {x : F p} :
+  x.toZMod varStore = [varStore|x]
+:= rfl
+
+@[simp, grind =]
+lemma eval_ofZMod {varStore : VarStore p} {v : ZMod p} :
+  [varStore|ofZMod p v] = .some v
+:= by simp [ofZMod]
+
+namespace ofZMod
+
+lemma isAlwaysValid (v : ZMod p) : F.isAlwaysValid (F.ofZMod p v) := by
+  unfold F.isAlwaysValid F.isValid F.ofZMod
+  simp
+
+end ofZMod
+
 instance : Convert p (F p) (ZMod p) where
-  toIdeal Γ x := x.eval Γ
-  toRepresents v := .c v
-  someOfIsValid := fun _ _ h ↦ h
-  toIdealtoRepresents := fun _ _ ↦ by simp [FixedExp.eval]
-  toRepresentstoIdeal := fun Γ x h ↦ by simp [FixedExp.eval, Option.some_get]
+  toIdeal Γ x := F.toZMod x Γ
+  toRepresents := F.ofZMod p
+  isValid_iff_isSome_toIdeal := fun _ _ ↦ Iff.rfl
+  toIdeal_toRepresents := fun _ _ ↦ by simp
+  toRepresents_toIdeal := fun Γ x _ ↦ by simp [Option.some_get]
+
+@[simp, grind =]
+lemma toIdeal_def {varStore : VarStore p} {x : F p} :
+  Convert.toIdeal varStore x = [varStore|x]
+:= rfl
+
+lemma toRepresents_def {v : ZMod p} :
+  Convert.toRepresents p (representsT := F p) (idealT := ZMod p) v = F.ofZMod p v
+:= rfl
+
+lemma eval_ofZMod_toZMod_of_isValid
+  {varStore : VarStore p} {x : F p} (h : x.isValid varStore)
+:
+  [varStore|(F.ofZMod p ((x.toZMod varStore).get h)) =Γ x]
+:= by simp [Option.some_get]
+
+section
+variable {p : ℕ} [NeZero p]
+
+def toFin (x : F p) (varStore : VarStore p) : Option (Fin p) :=
+  (x.eval varStore).map (ZMod.finEquiv p).symm
+
+def ofFin (p : ℕ) [NeZero p] (n : Fin p) : F p := .c ((ZMod.finEquiv p) n)
+
+@[simp, grind =]
+lemma toFin_def {varStore : VarStore p} {x : F p} :
+  x.toFin varStore = (x.eval varStore).map (ZMod.finEquiv p).symm
+:= rfl
+
+@[simp, grind =]
+lemma eval_ofFin {varStore : VarStore p} {n : Fin p} :
+  [varStore|ofFin p n] = .some ((ZMod.finEquiv p) n)
+:= by simp [ofFin]
+
+instance : Convert p (F p) (Fin p) where
+  toIdeal Γ x := F.toFin x Γ
+  toRepresents := F.ofFin p
+  isValid_iff_isSome_toIdeal Γ x := by unfold_projs; simp [F.isValid, F.toFin]
+  toIdeal_toRepresents Γ n := by simp [F.toFin, F.ofFin]
+  toRepresents_toIdeal Γ x h := by simp [F.toFin, F.ofFin, Option.some_get]
+
+lemma toIdeal_def_fin {varStore : VarStore p} {x : F p} :
+  Convert.toIdeal (representsT := F p) (idealT := Fin p) varStore x = F.toFin x varStore
+:= rfl
+
+lemma toRepresents_def_fin {n : Fin p} :
+  Convert.toRepresents p (representsT := F p) (idealT := Fin p) n = F.ofFin p n
+:= rfl
+
+end
 
 end F
 
