Clap/Lang/F/conditionalSwap.lean
@@ -3,16 +3,16 @@ import Clap.Lang.FB.FB
 
 namespace Clap.Edsl.Lang.F
 
-def conditionalSwap {p : ℕ} [Fact (p ≥ 2)] (sel : FB p) (a b : F p) : F p :=
+def conditionalSwap {p : ℕ} [Fact (p ≥ 2)] [p.AtLeastTwo] (sel : FB p) (a b : F p) : F p :=
   (a - b) * sel + b
 
 namespace conditionalSwap
 
 /-- selects `a` when `sel = 1` and `b` when `sel = 0` -/
-def spec (p : ℕ) [Fact (p ≥ 2)] : Prop :=
+def spec (p : ℕ) [Fact (p ≥ 2)] [p.AtLeastTwo] : Prop :=
   matchesTernaryFunction p (fun (s : Bool) (a b : ZMod p) ↦ if s then a else b) (conditionalSwap (p := p))
 
-lemma equiv (p : ℕ) [Fact (p ≥ 2)] : spec p := by sorry
+lemma equiv (p : ℕ) [Fact (p ≥ 2)] [p.AtLeastTwo] : spec p := by sorry
 
 end conditionalSwap
 
