Clap/eDSLState/Varstore.lean
@@ -12,4 +12,14 @@ instance {p : ℕ} : GetElem? (VarStore p) ℕ (ZMod p) (λ Γ x ↦ Γ.contains
   getElem  Γ x h := Γ.get x h
   getElem? Γ x   := Γ.get? x
 
+@[simp, grind =]
+lemma VarStore.getElem?_insert_self {p : ℕ} {Γ : VarStore p} {k : ℕ} {v : ZMod p} :
+  (Γ.insert k v)[k]? = some v
+:= Std.ExtTreeMap.getElem?_insert_self
+
+@[simp, grind =]
+lemma VarStore.get?_insert_self {p : ℕ} {Γ : VarStore p} {k : ℕ} {v : ZMod p} :
+  (Γ.insert k v).get? k = some v
+:= Std.ExtTreeMap.getElem?_insert_self
+
 end Clap
